Treat return values of new() as symbolic
We now treat the addresses of new() as any symbolic variables that may be
coerced into any other type of value (except that they don't collide and are
not errors). Since in the underlying semantics, new returns an arbitrary
bitstring, we could use the returned bitstring as a non-reference as well.

This also has the effect that we can use new(){} for random number generation.

src/Quivela/Language.hs
@@ -10,6 +10,7 @@
 {-# LANGUAGE LambdaCase #-}
 {-# LANGUAGE StandaloneDeriving #-}
 {-# LANGUAGE TypeFamilies #-}
+{-# LANGUAGE PatternSynonyms #-}
 module Quivela.Language where
 
 import Control.Applicative ((<$>))
@@ -61,9 +62,14 @@ data SymValue = SymVar String Type
   | Div Value Value
   | Le Value Value
   | ITE Prop Value Value
-  | SymRef String
+  | SymRef String -- FIXME: check if we can remove these and use refs for everything
+  | Ref Addr
   | Deref Value String
   deriving (Eq, Read, Show, Ord, Data, Typeable, Generic)
+
+-- Since we pattern-match repeatedly on references in various places, we define
+-- a pattern synonym that handles the fact that references are actually symbolic
+pattern VRef a = Sym (Ref a)
 
 -- | Quivela values
 data Value = VInt Integer
@@ -71,7 +77,6 @@ data Value = VInt Integer
   | VTuple [Value]
   | VError
   | VNil
-  | VRef Addr
   | Sym { _symVal :: SymValue }
   deriving (Eq, Read, Show, Ord, Data, Typeable, Generic)
 
